code/bignum/Hacl.Spec.Bignum.AlmostMontExponentiation.fst
@@ -107,7 +107,7 @@ let bn_exp_almost_mont_st (t:limb_t) (len:BN.bn_len t) =
   -> mu:limb t{BM.bn_mont_pre n mu}
   -> aM:ME.bn_mont_t n
   -> bBits:size_nat
-  -> b:lbignum t (blocks bBits (bits t)){bn_v b < pow2 bBits} ->
+  -> b:lbignum t (blocks0 bBits (bits t)){bn_v b < pow2 bBits} ->
   Pure (lbignum t len)
   (requires True)
   (ensures  fun resM ->
