code/bignum/Hacl.Spec.Bignum.Exponentiation.fsti
@@ -17,7 +17,7 @@ let bn_mod_exp_pre
   (n:lbignum t len)
   (a:lbignum t len)
   (bBits:size_nat)
-  (b:lbignum t (blocks bBits (bits t)))
+  (b:lbignum t (blocks0 bBits (bits t)))
  =
    bn_v n % 2 = 1 /\ 1 < bn_v n /\
    bn_v b < pow2 bBits /\ bn_v a < bn_v n
@@ -29,7 +29,7 @@ let bn_mod_exp_post
   (n:lbignum t len)
   (a:lbignum t len)
   (bBits:size_nat)
-  (b:lbignum t (blocks bBits (bits t)))
+  (b:lbignum t (blocks0 bBits (bits t)))
   (res:lbignum t len)
  =
   bn_mod_exp_pre n a bBits b /\
@@ -42,7 +42,7 @@ val bn_check_mod_exp:
   -> n:lbignum t len
   -> a:lbignum t len
   -> bBits:size_nat
-  -> b:lbignum t (blocks bBits (bits t)) ->
+  -> b:lbignum t (blocks0 bBits (bits t)) ->
   res:limb t{
     let b =
       bn_v n % 2 = 1 && 1 < bn_v n &&
@@ -57,7 +57,7 @@ let bn_mod_exp_precomp_st (t:limb_t) (len:BN.bn_len t) =
   -> r2:lbignum t len
   -> a:lbignum t len
   -> bBits:size_nat
-  -> b:lbignum t (blocks bBits (bits t)) ->
+  -> b:lbignum t (blocks0 bBits (bits t)) ->
   Pure (lbignum t len)
   (requires
     bn_mod_exp_pre n a bBits b /\
@@ -87,7 +87,7 @@ let bn_mod_exp_precompr2_st (t:limb_t) (len:BN.bn_len t) =
   -> r2:lbignum t len
   -> a:lbignum t len
   -> bBits:size_nat
-  -> b:lbignum t (blocks bBits (bits t)) ->
+  -> b:lbignum t (blocks0 bBits (bits t)) ->
   Pure (lbignum t len)
   (requires
     bn_mod_exp_pre n a bBits b /\
@@ -105,7 +105,7 @@ let bn_mod_exp_st (t:limb_t) (len:BN.bn_len t) =
   -> n:lbignum t len
   -> a:lbignum t len
   -> bBits:size_nat
-  -> b:lbignum t (blocks bBits (bits t)) ->
+  -> b:lbignum t (blocks0 bBits (bits t)) ->
   Pure (lbignum t len)
   (requires
     bn_mod_exp_pre n a bBits b /\
